Finish formalization of term equivalence and all related proofs.

theories/lang_oadt/equivalence.v
@@ -3,7 +3,6 @@ From oadt Require Import lang_oadt.syntax.
 From oadt Require Import lang_oadt.semantics.
 From oadt Require Import lang_oadt.typing.
 From oadt Require Import lang_oadt.infrastructure.
-From oadt Require Import lang_oadt.inversion.
 
 (** * Expression Equivalence *)
 (** Lemmas for expression equivalence. *)
@@ -12,17 +11,542 @@ Import syntax.notations.
 Import semantics.notations.
 Import typing.notations.
 
-Implicit Types (x X y Y : atom) (L : aset).
-Implicit Types (b : bool).
+Implicit Types (b : bool) (x X y Y : atom) (L : aset).
 
 #[local]
 Coercion EFVar : atom >-> expr.
+
+Section equivalence.
+
+Context (Σ : gctx).
+Context (Hwf : gctx_wf Σ).
+
+Notation "e '==>!' e'" := (Σ ⊢ e ==>! e')
+                            (at level 40,
+                             e' constr at level 0).
+
+Lemma pared_oval v e :
+  oval v ->
+  v ==>! e ->
+  v = e.
+Proof.
+  intros H. revert e.
+  induction H; intros ?; inversion 1; intros; subst; eauto; hauto.
+Qed.
+
+Lemma pared_otval ω τ :
+  otval ω ->
+  ω ==>! τ ->
+  ω = τ.
+Proof.
+  intros H. revert τ.
+  induction H; intros ?; inversion 1; intros; subst; eauto; hauto.
+Qed.
+
+
+(** ** Renaming Lemmas *)
+
+(* Technically [lc e1] should imply [lc e1'], but I have this assumption for
+convenience. *)
+Lemma pared_subst1_ e s s' x :
+  lc s -> lc s' ->
+  lc e ->
+  s ==>! s' ->
+  <{ {x↦s}e }> ==>! <{ {x↦s'}e }>.
+Proof.
+  intros ??.
+  induction 1; intros; simpl; try case_decide; eauto with pared;
+    econstructor; eauto with lc;
+      simpl_cofin?;
+      rewrite <- !subst_open_comm by (eauto; fast_set_solver!!); eauto.
+Qed.
+
+Lemma pared_subst1 e s s' x :
+  s ==>! s' ->
+  lc e ->
+  <{ {x↦s}e }> ==>! <{ {x↦s'}e }>.
+Proof.
+  intros. eapply pared_subst1_; qauto use: pared_lc.
+Qed.
+
+Lemma pared_subst_ e e' s s' x :
+  lc s -> lc s' ->
+  e ==>! e' ->
+  s ==>! s' ->
+  <{ {x↦s}e }> ==>! <{ {x↦s'}e' }>.
+Proof.
+  intros ??.
+  induction 1; intros; simpl; eauto using pared_subst1;
+    (* Massage the goal so the induction hypotheses can be applied. *)
+    rewrite ?subst_ite_distr;
+    rewrite ?subst_open_distr by assumption;
+    repeat match goal with
+           | H : oval ?v |- _ =>
+             rewrite !(subst_fresh v) by shelve
+           | H : otval ?ω |- _ =>
+             rewrite !(subst_fresh ω) by shelve
+           end;
+    econstructor; simpl_cofin?;
+      (* Apply induction hypotheses first before solving other side
+      conditions. *)
+      lazymatch goal with
+      | |- _ ==>! _ =>
+        rewrite <- ?subst_open_comm by (eauto; shelve);
+          auto_apply
+      | _ => idtac
+      end; eauto;
+        repeat lazymatch goal with
+               | |- _ !! _ = Some _ =>
+                 rewrite subst_fresh by shelve; eauto
+               | |- ovalty _ _ =>
+                 rewrite subst_fresh by shelve; eauto
+               | |- lc _ =>
+                 eauto using subst_lc
+               end; eauto.
+
+  Unshelve.
+
+  all : try fast_set_solver!!; simpl_fv; fast_set_solver*!!.
+Qed.
+
+Lemma pared_subst e e' s s' x :
+  e ==>! e' ->
+  s ==>! s' ->
+  <{ {x↦s}e }> ==>! <{ {x↦s'}e' }>.
+Proof.
+  qauto use: pared_subst_, pared_lc.
+Qed.
+
+Lemma pared_open e e' s s' x :
+  <{ e^x }> ==>! <{ e'^x }> ->
+  s ==>! s' ->
+  x ∉ fv e ∪ fv e' ->
+  <{ e^s }> ==>! <{ e'^s'}>.
+Proof.
+  intros.
+  rewrite (subst_intro e _ x) by fast_set_solver!!.
+  rewrite (subst_intro e' _ x) by fast_set_solver!!.
+  eapply pared_subst; eauto.
+Qed.
+
+Lemma pared_open1 e s s' :
+  s ==>! s' ->
+  lc <{ e^s }> ->
+  <{ e^s }> ==>! <{ e^s'}>.
+Proof.
+  intros.
+  destruct (exist_fresh (fv e)) as [x ?].
+  unshelve eapply pared_open; eauto.
+  constructor. eauto using open_respect_lc, pared_lc1 with lc.
+  fast_set_solver!!.
+Qed.
+
+Lemma pared_rename e e' x y :
+  <{ e^x }> ==>! <{ e'^x }> ->
+  x ∉ fv e ∪ fv e' ->
+  <{ e^y }> ==>! <{ e'^y }>.
+Proof.
+  intros.
+  eapply pared_open; eauto with lc.
+  econstructor; eauto with lc.
+Qed.
+
+(** ** Admissible Rules *)
+
+Ltac intro_solver :=
+  intros; econstructor; eauto; simpl_cofin;
+    eapply pared_rename; eauto; try fast_set_solver!!.
+
+Lemma ROCase_intro b ω1 ω2 v v1 v2 e1 e2 e1' e2' x :
+  <{ e1^x }> ==>! <{ e1'^x }> ->
+  <{ e2^x }> ==>! <{ e2'^x }> ->
+  oval v ->
+  ovalty v1 ω1 -> ovalty v2 ω2 ->
+  x ∉ fv e1 ∪ fv e1' ∪ fv e2 ∪ fv e2' ->
+  <{ ~case [inj@b<ω1 ~+ ω2> v] of e1 | e2 }> ==>!
+    <{ ~if [b] then (ite b (e1'^v) (e1'^v1)) else (ite b (e2'^v2) (e2'^v)) }>.
+Proof.
+  intro_solver.
+Qed.
+
+Lemma RApp_intro τ e1 e2 e1' e2' x :
+  e1 ==>! e1' ->
+  <{ e2^x }> ==>! <{ e2'^x }> ->
+  lc τ ->
+  x ∉ fv e2 ∪ fv e2' ->
+  <{ (\:τ => e2) e1 }> ==>! <{ e2'^e1' }>.
+Proof.
+  intro_solver.
+Qed.
+
+Lemma RLet_intro e1 e2 e1' e2' x :
+  e1 ==>! e1' ->
+  <{ e2^x }> ==>! <{ e2'^x }> ->
+  x ∉ fv e2 ∪ fv e2' ->
+  <{ let e1 in e2 }> ==>! <{ e2'^e1' }>.
+Proof.
+  intro_solver.
+Qed.
+
+Lemma RCase_intro b τ e0 e1 e2 e0' e1' e2' x:
+  e0 ==>! e0' ->
+  <{ e1^x }> ==>! <{ e1'^x }> ->
+  <{ e2^x }> ==>! <{ e2'^x }> ->
+  lc τ ->
+  x ∉ fv e1 ∪ fv e1' ∪ fv e2 ∪ fv e2' ->
+  <{ case inj@b<τ> e0 of e1 | e2 }> ==>! <{ ite b (e1'^e0') (e2'^e0') }>.
+Proof.
+  intro_solver.
+Qed.
+
+Lemma RCongPi_intro τ1 τ2 τ1' τ2' x :
+  τ1 ==>! τ1' ->
+  <{ τ2^x }> ==>! <{ τ2'^x }> ->
+  x ∉ fv τ2 ∪ fv τ2' ->
+  <{ Π:τ1, τ2 }> ==>! <{ Π:τ1', τ2' }>.
+Proof.
+  intro_solver.
+Qed.
+
+Lemma RCongAbs_intro τ e τ' e' x :
+  τ ==>! τ' ->
+  <{ e^x }> ==>! <{ e'^x }> ->
+  x ∉ fv e ∪ fv e' ->
+  <{ \:τ => e }> ==>! <{ \:τ' => e' }>.
+Proof.
+  intro_solver.
+Qed.
+
+Lemma RCongCase_intro l e0 e1 e2 e0' e1' e2' x :
+  e0 ==>! e0' ->
+  <{ e1^x }> ==>! <{ e1'^x }> ->
+  <{ e2^x }> ==>! <{ e2'^x }> ->
+  x ∉ fv e1 ∪ fv e1' ∪ fv e2 ∪ fv e2' ->
+  <{ case{l} e0 of e1 | e2 }> ==>! <{ case{l} e0' of e1' | e2' }>.
+Proof.
+  intro_solver.
+Qed.
+
+(** ** Inversion Lemmas *)
+
+Ltac inv_solver :=
+  inversion 1; subst; try apply_lc_inv; repeat esplit; eauto with pared.
+
+Lemma pared_inv_abs τ e t :
+  <{ \:τ => e }> ==>! t ->
+  exists τ' e' L,
+    t = <{ \:τ' => e' }> /\
+    τ ==>! τ' /\
+    (forall x, x ∉ L -> <{ e^x }> ==>! <{ e'^x }>).
+Proof.
+  inv_solver.
+Qed.
+
+Lemma pared_inv_pair e1 e2 t :
+  <{ (e1, e2) }> ==>! t ->
+  exists e1' e2',
+    t = <{ (e1', e2') }> /\
+    e1 ==>! e1' /\
+    e2 ==>! e2'.
+Proof.
+  inv_solver.
+Qed.
+
+Lemma pared_inv_fold X e t :
+  <{ fold<X> e }> ==>! t ->
+  exists e',
+    t = <{ fold<X> e' }> /\
+    e ==>! e'.
+Proof.
+  inv_solver.
+Qed.
+
+Lemma pared_inv_inj b τ e t :
+  <{ inj@b<τ> e }> ==>! t ->
+  exists τ' e',
+    t = <{ inj@b<τ'> e' }> /\
+    τ ==>! τ' /\
+    e ==>! e'.
+Proof.
+  inv_solver.
+Qed.
+
+End equivalence.
+
+Ltac pared_intro_ e :=
+  match e with
+  | <{ (\:_ => _) _ }> => eapply RApp_intro
+  | <{ ~case [inj@_<_> _] of _ | _ }> => eapply ROCase_intro
+  | <{ let _ in _ }> => eapply RLet_intro
+  | <{ case inj@_<_> _ of _ | _ }> => eapply RCase_intro
+  | <{ Π:_, _ }> => eapply RCongPi_intro
+  | <{ \:_ => _ }> => eapply RCongAbs_intro
+  | <{ case{_} _ of _ | _ }> => eapply RCongCase_intro
+  | _ => econstructor
+  end.
+
+Ltac pared_intro :=
+  match goal with
+  | |- _ ⊢ ?e ==>! _ => pared_intro_ e
+  end.
+
+Ltac apply_pared_inv_ e H :=
+  match e with
+  | <{ \:_ => _ }> => apply pared_inv_abs in H; try simp_hyp H
+  | <{ (_, _) }> => apply pared_inv_pair in H; try simp_hyp H
+  | <{ fold<_> _ }> => apply pared_inv_fold in H; try simp_hyp H
+  | <{ inj@_<_> _ }> => apply pared_inv_inj in H; try simp_hyp H
+  | _ => head_constructor e; sinvert H
+  end.
+
+Ltac apply_pared_inv :=
+  match goal with
+  | H : _ ⊢ ?e ==>! _ |- _ => apply_pared_inv_ e H
+  end; subst; eauto.
+
+Tactic Notation "lcrefl" "by" tactic3(tac) := eapply RRefl; tac.
+Tactic Notation "lcrefl" := lcrefl by eauto with lc.
+
+(** ** Confluence *)
+
+Section equivalence.
+
+Context (Σ : gctx).
+Context (Hwf : gctx_wf Σ).
+
+Notation "e '==>!' e'" := (Σ ⊢ e ==>! e')
+                            (at level 40,
+                             e' constr at level 0).
+Notation "e '==>*' e'" := (Σ ⊢ e ==>* e')
+                            (at level 40,
+                             e' custom oadt at level 99).
+Notation "e ≡ e'" := (Σ ⊢ e ≡ e').
+
+Lemma pared_diamond e e1 e2 :
+  e ==>! e1 ->
+  e ==>! e2 ->
+  exists e',
+    e1 ==>! e' /\
+    e2 ==>! e'.
+Proof.
+  intros H. revert e2.
+  induction H; intros;
+    repeat apply_pared_inv;
+    try apply_gctx_wf; simplify_map_eq;
+      (* Massage hypotheses related to oblivious values. *)
+      try select! (oval _)
+          (fun H => dup_hyp H (fun H => apply oval_lc in H));
+      try select! (otval _)
+          (fun H => dup_hyp H (fun H => apply otval_lc in H));
+      try select! (ovalty _ _)
+          (fun H => dup_hyp H (fun H => apply ovalty_lc in H; destruct H));
+      repeat
+        match goal with
+        | H : oval ?v, H' : ?v ==>! _ |- _ =>
+          eapply pared_oval in H'; [| solve [ eauto ] ]
+        | H : otval ?ω, H' : ?ω ==>! _ |- _ =>
+          eapply pared_otval in H'; [| solve [ eauto ]]
+        end; subst;
+        (* Solve some easy cases. *)
+        try solve [ repeat esplit; eauto;
+                    econstructor; eauto with lc ];
+        (* Generate local closure assumptions to avoid reproving the same
+        stuff. *)
+        repeat apply_lc_inv;
+        simpl_cofin?;
+          (* Generate more local closure assumptions. *)
+          try select! (_ ==>! _)
+              (fun H => match type of H with
+                      | _ ==>! ?e =>
+                        try assert (lc e) by eauto using pared_lc2
+                      end);
+          (* Use induction hypotheses. *)
+          repeat
+            match goal with
+            | H : context [exists _, ?u ==>! _ /\ _] |- _ =>
+              let e := fresh "e" in
+              let H1 := fresh "H" in
+              let H2 := fresh "H" in
+              edestruct H as [e [H1 H2]]; [
+                (* Discharge assumptions in the induction hypotheses. *)
+                try match goal with
+                    | |- ?e ==>! _ => head_constructor e; pared_intro
+                    end;
+                (* Be careful to not generate the useless induction
+                hypotheses. *)
+                try match goal with
+                    | H : ?e ==>! ?e' |- ?e ==>! _ =>
+                      lazymatch u with
+                      | context [e'] => fail
+                      | _ => apply H
+                      end
+                    end; solve [ eauto ]
+               |];
+              clear H;
+              try assert (lc e) by eauto using pared_lc2;
+              let go H :=
+                  lazymatch type of H with
+                  | ?e' ==>! _ =>
+                    (* Massage the parallel reduction assumptions to the right
+                    form. *)
+                    try lazymatch e' with
+                        | <{ ?e'^(fvar ?x) }> =>
+                          rewrite <- (open_close e x) in H by assumption
+                        end
+                  end
+              in go H1; go H2
+            end;
+    (* May invert some generated induction hypotheses. *)
+    repeat apply_pared_inv;
+    (* Solve more easy cases. *)
+    try solve [ try case_split; repeat esplit; eauto;
+                econstructor; eauto with lc ];
+    (* Solve the trickier cases. *)
+    let go _ :=
+        lazymatch goal with
+        | |- ?e ==>! ?e' =>
+          eauto;
+            match e with
+            | <{ _^?e2 }> =>
+              eapply pared_open; [ assumption
+                                 | solve [eauto] || lcrefl
+                                 | solve [eauto] || lcrefl
+                                 | .. ]
+            | _ => head_constructor e; pared_intro
+            | _ => lcrefl
+            end
+        end;
+          lazymatch goal with
+          | |- _ ∉ _ => shelve
+          | |- lc _ =>
+            eauto using typing_lc, kinding_lc with lc
+          | |- _ => eauto
+          end
+    in try solve [ repeat esplit; go ()
+                 | case_split; repeat esplit; do 2 go ()
+                 (* Sometimes I have to solve the right hand side first. *)
+                 | repeat esplit; cycle 1;
+                   solve [ do 2 go ()
+                         | case_split; do 2 go () ] ].
+
+  (* Application of abstraction. *)
+  match goal with
+  | H : context [exists _, <{ \:_ => ?e }> ==>! _ /\ _] |- _ =>
+    (* Avoid generating useless hypothesis. *)
+    match goal with
+    | H : _ ==>! ?e' |- _ =>
+      lazymatch e' with
+      | context [e] => clear H
+      end
+    end;
+      edestruct H as [? [??]]; [
+        pared_intro; eauto; set_shelve
+       |]
+  end.
+  repeat apply_pared_inv.
+  simpl_cofin.
+  repeat esplit; [ pared_intro | eapply pared_open ];
+    eauto; set_shelve.
+
+  Unshelve.
+  all : eauto; rewrite ?close_fv by eauto; fast_set_solver!!.
+Qed.
+
+Lemma pared_confluence_ e e1 e2 :
+  e ==>* e1 ->
+  e ==>! e2 ->
+  exists e',
+    e1 ==>! e' /\
+    e2 ==>* e'.
+Proof.
+  intros H. revert e2.
+  induction H; intros.
+  - match goal with
+      | H : _ ==>! _, H' : _ ==>! _ |- _ =>
+        edestruct pared_diamond as [? [??]];
+          [ apply H | apply H' | .. ]
+      end.
+    hauto use: rt_step.
+  - hauto use: rt_step.
+  - repeat match goal with
+           | H : forall e', ?e ==>! e' -> _, H' : ?e ==>! _ |- _ =>
+               edestruct H as [? [??]]; eauto; clear H
+           end.
+    hauto use: rt_trans.
+Qed.
+
+Lemma pared_confluence e e1 e2 :
+  e ==>* e1 ->
+  e ==>* e2 ->
+  exists e',
+    e1 ==>* e' /\
+    e2 ==>* e'.
+Proof.
+  intros H. revert e2.
+  induction H; intros.
+  - edestruct pared_confluence_ as [? [??]]; eauto.
+    hauto use: rt_step.
+  - hauto use: rt_step.
+  - repeat match goal with
+           | H : forall e', ?e ==>* e' -> _, H' : ?e ==>* _ |- _ =>
+               edestruct H as [? [??]]; eauto; clear H
+           end.
+    hauto use: rt_trans.
+Qed.
+
+Lemma pared_equiv_iff_join e1 e2 :
+  e1 ≡ e2 <-> pared_equiv_join Σ e1 e2.
+Proof.
+  split.
+  - induction 1;
+      hauto ctrs: pared_equiv_join, clos_refl_trans, pared inv: pared_equiv_join.
+  - intros [].
+    (* Another equivalent definition of the closure is easier in this case. *)
+    repeat match goal with
+           | H : _ ==>* _ |- _ =>
+             apply clos_rt_rt1n in H
+           end.
+
+    select (clos_refl_trans_1n _ _ _ _) (fun H => induction H);
+        try hauto ctrs: pared_equiv.
+    select (clos_refl_trans_1n _ _ _ _) (fun H => induction H);
+      hauto ctrs: pared_equiv.
+Qed.
+
+(** [pared_equiv] is an equivalence *)
+
+#[global]
+Instance pared_equiv_is_refl : Reflexive (pared_equiv Σ).
+Proof.
+  hnf; intros; econstructor.
+Qed.
+
+#[global]
+Instance pared_equiv_is_symm : Symmetric (pared_equiv Σ).
+Proof.
+  hnf; intros; srewrite pared_equiv_iff_join;
+    hauto ctrs: pared_equiv_join inv: pared_equiv_join.
+Qed.
+
+#[global]
+Instance pared_equiv_is_trans : Transitive (pared_equiv Σ).
+Proof.
+  hnf. intros ??? H1 H2.
+  srewrite pared_equiv_iff_join.
+  destruct H1 as [e1 e e1'].
+  destruct H2 as [e e2 e2'].
+  edestruct (pared_confluence e e1' e2') as [? [??]]; eauto.
+  econstructor; eapply rt_trans; eauto.
+Qed.
+
+(* Is there a conventional way to achieve this? *)
+Hint Extern 0 (gctx_wf _) => eassumption : typeclass_instances.
 
 (** ** Weak head normal form *)
 (** I only use weak head normal form as a machinery for proofs right now, so
 only the necessary cases (for types) are defined. But I may extend it with other
 expressions later. *)
-Inductive whnf {Σ : gctx} : expr -> Prop :=
+Inductive whnf : expr -> Prop :=
 | WUnitT : whnf <{ 𝟙 }>
 | WBool{l} : whnf <{ 𝔹{l} }>
 | WPi τ1 τ2 : whnf <{ Π:τ1, τ2 }>
@@ -32,97 +556,265 @@ Inductive whnf {Σ : gctx} : expr -> Prop :=
     Σ !! X = Some (DADT τ) ->
     whnf <{ gvar X }>
 .
-Arguments whnf : clear implicits.
-Hint Constructors whnf : whnf.
 
 (** Type equivalence for the weak head normal form fragments. This relation
 always assumes that the two arguments are already in [whnf]. *)
-Inductive whnf_equiv {Σ : gctx} : expr -> expr -> Prop :=
+Inductive whnf_equiv : expr -> expr -> Prop :=
 | WQUnitT : whnf_equiv <{ 𝟙 }> <{ 𝟙 }>
 | WQBool l : whnf_equiv <{ 𝔹{l} }> <{ 𝔹{l} }>
 | WQPi τ1 τ2 τ1' τ2' L :
-    Σ ⊢ τ1 ≡ τ1' ->
-    (forall x, x ∉ L -> Σ ⊢ τ2^x ≡ τ2'^x) ->
+    τ1 ≡ τ1' ->
+    (forall x, x ∉ L -> <{ τ2^x }> ≡ <{ τ2'^x }>) ->
     whnf_equiv <{ Π:τ1, τ2 }> <{ Π:τ1', τ2' }>
 | WQProd τ1 τ2 τ1' τ2' :
-    Σ ⊢ τ1 ≡ τ1' ->
-    Σ ⊢ τ2 ≡ τ2' ->
+    τ1 ≡ τ1' ->
+    τ2 ≡ τ2' ->
     whnf_equiv <{ τ1 * τ2 }> <{ τ1' * τ2' }>
 | WQSum l τ1 τ2 τ1' τ2' :
-    Σ ⊢ τ1 ≡ τ1' ->
-    Σ ⊢ τ2 ≡ τ2' ->
+    τ1 ≡ τ1' ->
+    τ2 ≡ τ2' ->
     whnf_equiv <{ τ1 +{l} τ2 }> <{ τ1' +{l} τ2' }>
 | WQADT X : whnf_equiv <{ gvar X }> <{ gvar X }>
-| WQInj b τ e τ' e' :
-    Σ ⊢ τ ≡ τ' ->
-    Σ ⊢ e ≡ e' ->
-    whnf_equiv <{ inj@b<τ> e }> <{ inj@b<τ'> e' }>
 .
-Arguments whnf_equiv : clear implicits.
-Hint Constructors whnf_equiv : whnf_equiv.
 
-(** ** Properties of type equivalence  *)
-Lemma expr_equiv_step Σ e e' :
-  Σ ⊨ e -->! e' ->
-  Σ ⊢ e ≡ e'.
+#[global]
+Instance whnf_equiv_is_symm : Symmetric whnf_equiv.
 Proof.
-  induction 1; try select (ectx _) (fun H => sinvert H);
-    eauto with expr_equiv.
-
-  (* Oblivious case *)
-  etrans; [ econstructor; eauto | ].
-  symmetry.
-  etrans; [ econstructor; eauto | ].
-  hauto.
-
-  (* Generated by the cofinite quantifiers. *)
-  Unshelve.
-  all : exact ∅.
+  hnf. induction 1; econstructor; simpl_cofin?; equiv_naive_solver.
 Qed.
 
-(* We may weaken it so Γ = ∅. But we need to weaken all theorems depending on
-it. *)
-Lemma expr_equiv_obliv_type_preserve_ Σ Γ τ τ' κ κ' :
-  gctx_wf Σ ->
-  Σ; Γ ⊢ τ :: κ ->
-  Σ; Γ ⊢ τ' :: κ' ->
-  Σ ⊢ τ ≡ τ' ->
-  κ ⊑ <{ *@O }> ->
-  Σ; Γ ⊢ τ' :: *@O.
+Lemma pared_whnf τ1 τ2 :
+  τ1 ==>! τ2 ->
+  whnf τ1 ->
+  whnf τ2.
 Proof.
-Admitted.
-
-Lemma expr_equiv_obliv_type_preserve Σ Γ τ τ' κ :
-  gctx_wf Σ ->
-  Σ; Γ ⊢ τ :: *@O ->
-  Σ ⊢ τ ≡ τ' ->
-  Σ; Γ ⊢ τ' :: κ ->
-  Σ; Γ ⊢ τ' :: *@O.
-Proof.
-  qauto use: expr_equiv_obliv_type_preserve_ solve: lattice_naive_solver.
+  induction 1; eauto; intros Hw;
+    try lazymatch type of Hw with
+        | whnf ?e =>
+          head_constructor e; sinvert Hw
+        end;
+    simplify_map_eq; try solve [econstructor].
 Qed.
 
-(** [whnf_equiv] is a faithful fragment of [expr_equiv]. *)
-Lemma expr_equiv_iff_whnf_equiv Σ τ1 τ2 :
-  whnf Σ τ1 -> whnf Σ τ2 ->
-  Σ ⊢ τ1 ≡ τ2 <->
-  whnf_equiv Σ τ1 τ2.
+Lemma pared_whnf_equiv τ1 τ1' τ2 :
+  τ1 ==>! τ1' ->
+  whnf τ1 ->
+  whnf_equiv τ1' τ2 ->
+  whnf_equiv τ1 τ2.
 Proof.
-Admitted.
+  intros H. revert τ2.
+  induction H; eauto; intros ? Hw;
+    try lazymatch type of Hw with
+        | whnf ?e =>
+          head_constructor e; sinvert Hw
+        end; intros;
+    simplify_map_eq;
+  select (whnf_equiv _ _) (fun H => sinvert H);
+  econstructor; simpl_cofin?;
+  eauto with pared_equiv.
+Qed.
 
-Lemma otval_whnf Σ ω :
+(** [whnf_equiv] refines [pared_equiv] under some side conditions. *)
+Lemma pared_equiv_whnf_equiv τ1 τ2 :
+  τ1 ≡ τ2 ->
+  whnf τ1 -> whnf τ2 ->
+  whnf_equiv τ1 τ2.
+Proof.
+  induction 1.
+  - intros [] []; econstructor; simpl_cofin?; equiv_naive_solver.
+  - hauto use: pared_whnf, pared_whnf_equiv.
+  - intros.
+    symmetry.
+    match goal with
+    | H : context [whnf_equiv _ _] |- _ => symmetry in H
+    end.
+    hauto use: pared_whnf, pared_whnf_equiv.
+Qed.
+
+Lemma otval_whnf ω :
   otval ω ->
-  whnf Σ ω.
+  whnf ω.
 Proof.
   induction 1; sfirstorder.
 Qed.
+
+(** [pared] refines [step]. *)
+Lemma pared_step e e' :
+  Σ ⊨ e -->! e' ->
+  lc e ->
+  e ==>! e'.
+Proof.
+  induction 1; intros; try select (ectx _) (fun H => sinvert H);
+    repeat apply_lc_inv;
+    repeat econstructor; eauto.
+Qed.
+
+Lemma pared_equiv_pared e e' :
+  e ==>! e' ->
+  e ≡ e'.
+Proof.
+  eauto with pared_equiv.
+Qed.
+
+Lemma pared_equiv_step e e' :
+  Σ ⊨ e -->! e' ->
+  lc e ->
+  e ≡ e'.
+Proof.
+  hauto use: pared_step, pared_equiv_pared.
+Qed.
+
+(** Substitution lemmas for [pared_equiv] *)
+Lemma pared_equiv_subst1 e s s' x :
+  s ≡ s' ->
+  lc e ->
+  {x↦s}e ≡ {x↦s'}e.
+Proof.
+  intros H ?.
+  induction H;
+    econstructor; solve [ eauto using pared_subst1 ].
+Qed.
+
+Lemma pared_equiv_subst2 e e' s x :
+  e ≡ e' ->
+  lc s ->
+  {x↦s}e ≡ {x↦s}e'.
+Proof.
+  intros H ?.
+  induction H; intros;
+    hauto ctrs: pared_equiv, pared using pared_subst.
+Qed.
+
+(* Different combinations of local closure conditions are possible. *)
+Lemma pared_equiv_subst e e' s s' x :
+  e ≡ e' ->
+  s ≡ s' ->
+  lc e ->
+  lc s' ->
+  {x↦s}e ≡ {x↦s'}e'.
+Proof.
+  intros.
+  etrans.
+  eapply pared_equiv_subst1; eauto.
+  eapply pared_equiv_subst2; eauto.
+Qed.
+
+Lemma pared_equiv_rename τ τ' x y :
+  τ ≡ τ' ->
+  {x↦y}τ ≡ {x↦y}τ'.
+Proof.
+  eauto using pared_equiv_subst2 with lc.
+Qed.
+
+(* A few alternative statements exist, e.g., having [x] as an argument. But this
+one is the most convenient. *)
+Lemma pared_equiv_open1 e s s' L :
+  s ≡ s' ->
+  (forall x, x ∉ L -> lc <{ e^x }>) ->
+  <{ e^s }> ≡ <{ e^s' }>.
+Proof.
+  intros.
+  simpl_cofin.
+  rewrite (subst_intro e s _) by fast_set_solver!!.
+  rewrite (subst_intro e s' _) by fast_set_solver!!.
+  eauto using pared_equiv_subst1.
+Qed.
+
+Lemma pared_equiv_open2 e e' s x :
+  <{ e^x }> ≡ <{ e'^x }> ->
+  lc s ->
+  x ∉ fv e ∪ fv e' ->
+  <{ e^s }> ≡ <{ e'^s }>.
+Proof.
+  intros.
+  rewrite (subst_intro e s x) by fast_set_solver!!.
+  rewrite (subst_intro e' s x) by fast_set_solver!!.
+  eauto using pared_equiv_subst2.
+Qed.
+
+Lemma pared_equiv_open e e' s s' x :
+  <{ e^x }> ≡ <{ e'^x }> ->
+  s ≡ s' ->
+  lc <{ e^x }> ->
+  lc s' ->
+  x ∉ fv e ∪ fv e' ->
+  <{ e^s }> ≡ <{ e'^s' }>.
+Proof.
+  intros.
+  rewrite (subst_intro e s x) by fast_set_solver!!.
+  rewrite (subst_intro e' s' x) by fast_set_solver!!.
+  eauto using pared_equiv_subst.
+Qed.
+
+(** ** Congruence Lemmas *)
+
+(* Another proof strategy is to reduce them to [pared_equiv_subst]. *)
+
+Ltac congr_solver :=
+  intros H1 H2; intros;
+    induction H1;
+    solve [ hauto ctrs: pared_equiv, pared use: pared_lc
+          | induction H2; hauto ctrs: pared_equiv, pared use: pared_lc ].
+
+Lemma pared_equiv_congr_prod τ1 τ1' τ2 τ2' :
+  τ1 ≡ τ1' ->
+  τ2 ≡ τ2' ->
+  lc τ1 ->
+  lc τ2 ->
+  lc τ2' ->
+  <{ τ1 * τ2 }> ≡ <{ τ1' * τ2' }>.
+Proof.
+  congr_solver.
+Qed.
+
+Lemma pared_equiv_congr_sum τ1 τ1' τ2 τ2' l :
+  τ1 ≡ τ1' ->
+  τ2 ≡ τ2' ->
+  lc τ1 ->
+  lc τ2 ->
+  lc τ2' ->
+  <{ τ1 +{l} τ2 }> ≡ <{ τ1' +{l} τ2' }>.
+Proof.
+  congr_solver.
+Qed.
+
+Lemma pared_equiv_congr_inj τ τ' e e' l b :
+  τ ≡ τ' ->
+  e ≡ e' ->
+  lc τ ->
+  lc e ->
+  lc e' ->
+  <{ inj{l}@b<τ> e }> ≡ <{ inj{l}@b<τ'> e' }>.
+Proof.
+  congr_solver.
+Qed.
+
+(* This is good enough for our purposes though it is weaker than it could be. *)
+Lemma pared_equiv_congr_pi τ1 τ1' τ2 x :
+  τ1 ≡ τ1' ->
+  lc <{ τ2^x }> ->
+  <{ Π:τ1, τ2 }> ≡ <{ Π:τ1', τ2 }>.
+Proof.
+  intros H; intros.
+  induction H;
+    econstructor;
+    solve [ eauto; econstructor; eauto;
+            simpl_cofin?; lcrefl by eauto using lc_rename ].
+Qed.
+
+End equivalence.
+
+Hint Constructors whnf : whnf.
+Hint Constructors whnf_equiv : whnf_equiv.
+
+Hint Extern 0 (gctx_wf _) => eassumption : typeclass_instances.
 
 (** Simplify type equivalence to [whnf_equiv]. Possibly derive contradiction if
 two equivalent types in [whnf] have different head. *)
 Tactic Notation "simpl_whnf_equiv" "by" tactic3(tac) :=
   match goal with
   | H : _ ⊢ ?τ1 ≡ ?τ2 |- _ =>
-    apply expr_equiv_iff_whnf_equiv in H;
+    apply pared_equiv_whnf_equiv in H;
     [ sinvert H
     | solve [tac]
     | solve [tac] ]
@@ -130,3 +822,11 @@ Tactic Notation "simpl_whnf_equiv" "by" tactic3(tac) :=
 
 Tactic Notation "simpl_whnf_equiv" :=
   simpl_whnf_equiv by eauto using otval_whnf with whnf.
+
+Ltac apply_pared_equiv_congr :=
+  lazymatch goal with
+  | |- _ ⊢ Π:_, _ ≡ Π: _, _ => eapply pared_equiv_congr_pi
+  | |- _ ⊢ _ * _ ≡ _ * _ => eapply pared_equiv_congr_prod
+  | |- _ ⊢ _ +{_} _ ≡ _ +{_} _ => eapply pared_equiv_congr_sum
+  | |- _ ⊢ inj{_}@_<_> _ ≡ inj{_}@_<_> _ => eapply pared_equiv_congr_inj
+  end.
