theories/lang_oadt/inversion.v
@@ -3,18 +3,24 @@ From oadt Require Import lang_oadt.syntax.
 From oadt Require Import lang_oadt.semantics.
 From oadt Require Import lang_oadt.typing.
 From oadt Require Import lang_oadt.infrastructure.
+From oadt Require Import lang_oadt.equivalence.
 
 Import syntax.notations.
 Import semantics.notations.
 Import typing.notations.
 
-Implicit Types (x X y Y : atom) (L : aset).
-Implicit Types (b : bool).
+Implicit Types (b : bool) (x X y Y : atom) (L : aset).
 
 #[local]
 Coercion EFVar : atom >-> expr.
 
+
 (** * Inversion Lemmas *)
+
+Section inversion.
+
+Context (Σ : gctx).
+Context (Hwf : gctx_wf Σ).
 
 (** ** Kind inversion  *)
 Tactic Notation "kind_inv_solver" "by" tactic3(tac) :=
@@ -27,7 +33,7 @@ Tactic Notation "kind_inv_solver" "by" tactic3(tac) :=
 Tactic Notation "kind_inv_solver" :=
   kind_inv_solver by (repeat esplit; eauto; lattice_naive_solver).
 
-Lemma kind_inv_pi Σ Γ τ1 τ2 κ :
+Lemma kind_inv_pi Γ τ1 τ2 κ :
   Σ; Γ ⊢ Π:τ1, τ2 :: κ ->
   κ = <{ *@M }> /\
   exists L κ1 κ2,
@@ -37,13 +43,13 @@ Proof.
   kind_inv_solver by sfirstorder use: top_inv.
 Qed.
 
-Lemma kind_inv_bool Σ Γ κ :
+Lemma kind_inv_bool Γ κ :
   Σ; Γ ⊢ 𝔹 :: κ -> <{ *@P }> ⊑ κ.
 Proof.
   kind_inv_solver.
 Qed.
 
-Lemma kind_inv_prod Σ Γ τ1 τ2 κ :
+Lemma kind_inv_prod Γ τ1 τ2 κ :
   Σ; Γ ⊢ τ1 * τ2 :: κ ->
   exists κ',
     Σ; Γ ⊢ τ1 :: κ' /\
@@ -53,7 +59,7 @@ Proof.
   kind_inv_solver.
 Qed.
 
-Lemma kind_inv_sum Σ Γ τ1 τ2 κ :
+Lemma kind_inv_sum Γ τ1 τ2 κ :
   Σ; Γ ⊢ τ1 + τ2 :: κ ->
   <{ *@P }> ⊑ κ /\
   exists κ',
@@ -64,7 +70,7 @@ Proof.
                            use: join_ub_r.
 Qed.
 
-Lemma kind_inv_osum Σ Γ τ1 τ2 κ :
+Lemma kind_inv_osum Γ τ1 τ2 κ :
   Σ; Γ ⊢ τ1 ~+ τ2 :: κ ->
   <{ *@O }> ⊑ κ /\
   Σ; Γ ⊢ τ1 :: *@O /\
@@ -73,14 +79,14 @@ Proof.
   kind_inv_solver.
 Qed.
 
-Lemma kind_inv_gvar Σ Γ X κ :
+Lemma kind_inv_gvar Γ X κ :
   Σ; Γ ⊢ gvar X :: κ ->
   <{ *@P }> ⊑ κ /\ exists τ, Σ !! X = Some (DADT τ).
 Proof.
   kind_inv_solver.
 Qed.
 
-Lemma kind_inv_app Σ Γ e1 e2 κ :
+Lemma kind_inv_app Γ e1 e2 κ :
   Σ; Γ ⊢ e1 e2 :: κ ->
   <{ *@O }> ⊑ κ /\
   exists X τ e',
@@ -91,7 +97,7 @@ Proof.
   kind_inv_solver.
 Qed.
 
-Lemma kind_inv_ite Σ Γ l e0 τ1 τ2 κ :
+Lemma kind_inv_ite Γ l e0 τ1 τ2 κ :
   Σ; Γ ⊢ if{l} e0 then τ1 else τ2 :: κ ->
   <{ *@O }> ⊑ κ /\
   l = low /\
@@ -102,7 +108,7 @@ Proof.
   kind_inv_solver.
 Qed.
 
-Lemma kind_inv_let Σ Γ e τ κ :
+Lemma kind_inv_let Γ e τ κ :
   Σ; Γ ⊢ let e in τ :: κ ->
   <{ *@O }> ⊑ κ /\
   exists τ' L,
@@ -112,7 +118,7 @@ Proof.
   kind_inv_solver.
 Qed.
 
-Lemma kind_inv_case Σ Γ l e0 τ1 τ2 κ :
+Lemma kind_inv_case Γ l e0 τ1 τ2 κ :
   Σ; Γ ⊢ case{l} e0 of τ1 | τ2 :: κ ->
   <{ *@O }> ⊑ κ /\
   l = low /\
@@ -124,59 +130,284 @@ Proof.
   kind_inv_solver.
 Qed.
 
-Lemma kind_inv_mux Σ Γ e0 e1 e2 κ :
+Lemma kind_inv_mux Γ e0 e1 e2 κ :
   Σ; Γ ⊢ ~if e0 then e1 else e2 :: κ -> False.
 Proof.
   kind_inv_solver.
 Qed.
 
-Lemma kind_inv_sec Σ Γ e κ :
+Lemma kind_inv_sec Γ e κ :
   Σ; Γ ⊢ s𝔹 e :: κ -> False.
 Proof.
   kind_inv_solver.
 Qed.
 
-Lemma kind_inv_pair Σ Γ e1 e2 κ :
+Lemma kind_inv_pair Γ e1 e2 κ :
   Σ; Γ ⊢ (e1, e2) :: κ -> False.
 Proof.
   kind_inv_solver.
 Qed.
 
-Lemma kind_inv_proj Σ Γ b e κ :
+Lemma kind_inv_proj Γ b e κ :
   Σ; Γ ⊢ π@b e :: κ -> False.
 Proof.
   kind_inv_solver.
 Qed.
 
-Lemma kind_inv_inj Σ Γ l b τ e κ :
+Lemma kind_inv_inj Γ l b τ e κ :
   Σ; Γ ⊢ inj{l}@b<τ> e :: κ -> False.
 Proof.
   kind_inv_solver.
 Qed.
 
-Lemma kind_inv_ocase Σ Γ e0 e1 e2 κ :
+Lemma kind_inv_ocase Γ e0 e1 e2 κ :
   Σ; Γ ⊢ ~case e0 of e1 | e2 :: κ -> False.
 Proof.
   kind_inv_solver.
 Qed.
 
-Lemma kind_inv_fold Σ Γ X e κ :
+Lemma kind_inv_fold Γ X e κ :
   Σ; Γ ⊢ fold<X> e :: κ -> False.
 Proof.
   kind_inv_solver.
 Qed.
 
-Lemma kind_inv_unfold Σ Γ X e κ :
+Lemma kind_inv_unfold Γ X e κ :
   Σ; Γ ⊢ unfold<X> e :: κ -> False.
 Proof.
   kind_inv_solver.
 Qed.
 
-Lemma kind_inv_abs Σ Γ τ e κ :
+Lemma kind_inv_abs Γ τ e κ :
   Σ; Γ ⊢ \:τ => e :: κ -> False.
 Proof.
   kind_inv_solver.
 Qed.
+
+(** ** Type inversion *)
+Tactic Notation "type_inv_solver" "by" tactic3(tac) :=
+  match goal with
+  | |- _; _ ⊢ ?e : _ -> _ => remember e
+  end;
+  induction 1; subst; simp_hyps; simplify_eq;
+  tac.
+
+Tactic Notation "type_inv_solver" :=
+  type_inv_solver by (repeat esplit; eauto; equiv_naive_solver).
+
+Lemma type_inv_unit Γ τ :
+  Σ; Γ ⊢ () : τ ->
+  Σ ⊢ τ ≡ 𝟙.
+Proof.
+  type_inv_solver.
+Qed.
+
+Lemma type_inv_lit Γ b τ :
+  Σ; Γ ⊢ lit b : τ ->
+  Σ ⊢ τ ≡ 𝔹.
+Proof.
+  type_inv_solver.
+Qed.
+
+Lemma type_inv_abs Γ e τ2 τ :
+  Σ; Γ ⊢ \:τ2 => e : τ ->
+  exists τ1 κ L,
+    Σ; Γ ⊢ τ2 :: κ /\
+    (forall x, x ∉ L -> Σ; (<[x:=τ2]> Γ) ⊢ e^x : τ1^x) /\
+    Σ ⊢ τ ≡ Π:τ2, τ1.
+Proof.
+  type_inv_solver.
+Qed.
+
+Lemma type_inv_gvar Γ x τ :
+  Σ; Γ ⊢ gvar x : τ ->
+  exists τ' e,
+    Σ !! x = Some (DFun τ' e) /\
+    Σ ⊢ τ ≡ τ'.
+Proof.
+  type_inv_solver.
+Qed.
+
+Lemma type_inv_pair Γ e1 e2 τ :
+  Σ; Γ ⊢ (e1, e2) : τ ->
+  exists τ1 τ2,
+    Σ; Γ ⊢ e1 : τ1 /\
+    Σ; Γ ⊢ e2 : τ2 /\
+    Σ ⊢ τ ≡ τ1 * τ2.
+Proof.
+  type_inv_solver.
+Qed.
+
+Lemma type_inv_inj Γ b e τ' τ :
+  Σ; Γ ⊢ inj@b<τ'> e : τ ->
+  exists τ1 τ2 κ,
+    τ' = <{ τ1 + τ2 }> /\
+    Σ; Γ ⊢ τ1 + τ2 :: κ /\
+    Σ; Γ ⊢ e : ite b τ1 τ2 /\
+    Σ ⊢ τ ≡ τ1 + τ2.
+Proof.
+  type_inv_solver.
+Qed.
+
+Lemma type_inv_oinj Γ b e τ' τ :
+  Σ; Γ ⊢ ~inj@b<τ'> e : τ ->
+  exists τ1 τ2,
+    τ' = <{ τ1 ~+ τ2 }> /\
+    Σ; Γ ⊢ τ1 ~+ τ2 :: *@O /\
+    Σ; Γ ⊢ e : ite b τ1 τ2 /\
+    Σ ⊢ τ ≡ τ1 ~+ τ2.
+Proof.
+  type_inv_solver.
+Qed.
+
+Lemma type_inv_fold Γ X e τ :
+  Σ; Γ ⊢ fold<X> e : τ ->
+  exists τ',
+    Σ; Γ ⊢ e : τ' /\
+    Σ !! X = Some (DADT τ') /\
+    Σ ⊢ τ ≡ gvar X.
+Proof.
+  type_inv_solver.
+Qed.
+
+Lemma type_inv_boxedlit Γ b τ :
+  Σ; Γ ⊢ [b] : τ ->
+  Σ ⊢ τ ≡ ~𝔹.
+Proof.
+  type_inv_solver.
+Qed.
+
+Lemma type_inv_boxedinj Γ b v ω τ :
+  Σ; Γ ⊢ [inj@b<ω> v] : τ ->
+  exists ω1 ω2,
+    ω = <{ ω1 ~+ ω2 }> /\
+    ovalty <{ [inj@b<ω> v] }> ω /\
+    Σ ⊢ τ ≡ ω1 ~+ ω2.
+Proof.
+  type_inv_solver by hauto lq: on solve: equiv_naive_solver
+                           ctrs: ovalty inv: ovalty.
+Qed.
+
+Lemma type_inv_case Γ e0 e1 e2 τ :
+  Σ; Γ ⊢ case e0 of e1 | e2 : τ ->
+  exists τ1 τ2 τ' κ L1 L2,
+    Σ; Γ ⊢ τ'^e0 :: κ /\
+    Σ; Γ ⊢ e0 : τ1 + τ2 /\
+    (forall x, x ∉ L1 -> Σ; (<[x:=τ1]> Γ) ⊢ e1^x : τ'^(inl<τ1 + τ2> x)) /\
+    (forall x, x ∉ L2 -> Σ; (<[x:=τ2]> Γ) ⊢ e2^x : τ'^(inr<τ1 + τ2> x)) /\
+    Σ ⊢ τ ≡ τ'^e0.
+Proof.
+  type_inv_solver.
+Qed.
+
+Lemma type_inv_ocase Γ e0 e1 e2 τ :
+  Σ; Γ ⊢ ~case e0 of e1 | e2 : τ ->
+  exists τ1 τ2 τ' L1 L2,
+    Σ; Γ ⊢ τ' :: *@O /\
+    Σ; Γ ⊢ e0 : τ1 ~+ τ2 /\
+    (forall x, x ∉ L1 -> Σ; (<[x:=τ1]> Γ) ⊢ e1^x : τ') /\
+    (forall x, x ∉ L2 -> Σ; (<[x:=τ2]> Γ) ⊢ e2^x : τ') /\
+    Σ ⊢ τ ≡ τ'.
+Proof.
+  type_inv_solver.
+Qed.
+
+Lemma type_inv_case_ Γ l e0 e1 e2 τ :
+  Σ; Γ ⊢ case{l} e0 of e1 | e2 : τ ->
+  exists τ1 τ2 τ' κ L1 L2,
+    Σ; Γ ⊢ τ' :: κ /\
+    Σ; Γ ⊢ e0 : τ1 +{l} τ2 /\
+    (forall x, x ∉ L1 -> exists τ', Σ; (<[x:=τ1]> Γ) ⊢ e1^x : τ') /\
+    (forall x, x ∉ L2 -> exists τ', Σ; (<[x:=τ2]> Γ) ⊢ e2^x : τ') /\
+    Σ ⊢ τ ≡ τ'.
+Proof.
+  type_inv_solver by (repeat (esplit; eauto); equiv_naive_solver).
+Qed.
+
+Lemma type_inv_prod Γ τ1 τ2 τ :
+  Σ; Γ ⊢ τ1 * τ2 : τ -> False.
+Proof.
+  type_inv_solver.
+Qed.
+
+Lemma type_inv_sum Γ l τ1 τ2 τ :
+  Σ; Γ ⊢ τ1 +{l} τ2 : τ -> False.
+Proof.
+  type_inv_solver.
+Qed.
+
+Lemma type_inv_app Γ e1 e2 τ :
+  Σ; Γ ⊢ e1 e2 : τ ->
+  exists τ1 τ2,
+    Σ; Γ ⊢ e1 : Π:τ2, τ1 /\
+    Σ; Γ ⊢ e2 : τ2 /\
+    Σ ⊢ τ ≡ τ1^e2.
+Proof.
+  type_inv_solver.
+Qed.
+
+Lemma type_inv_let Γ e1 e2 τ :
+  Σ; Γ ⊢ let e1 in e2 : τ ->
+  exists τ1 τ2 L,
+    Σ; Γ ⊢ e1 : τ1 /\
+    (forall x, x ∉ L -> Σ; (<[x:=τ1]> Γ) ⊢ e2^x : τ2^x) /\
+    Σ ⊢ τ ≡ τ2^e1.
+Proof.
+  type_inv_solver.
+Qed.
+
+Lemma type_inv_sec Γ e τ :
+  Σ; Γ ⊢ s𝔹 e : τ ->
+  Σ; Γ ⊢ e : 𝔹 /\
+  Σ ⊢ τ ≡ ~𝔹.
+Proof.
+  type_inv_solver.
+Qed.
+
+Lemma type_inv_ite Γ e0 e1 e2 τ :
+  Σ; Γ ⊢ if e0 then e1 else e2 : τ ->
+  exists τ' κ,
+    Σ; Γ ⊢ e0 : 𝔹 /\
+    Σ; Γ ⊢ e1 : τ'^(lit true) /\
+    Σ; Γ ⊢ e2 : τ'^(lit false) /\
+    Σ; Γ ⊢ τ'^e0 :: κ /\
+    Σ ⊢ τ ≡ τ'^e0.
+Proof.
+  type_inv_solver.
+Qed.
+
+Lemma type_inv_mux Γ e0 e1 e2 τ :
+  Σ; Γ ⊢ ~if e0 then e1 else e2 : τ ->
+  exists τ',
+    Σ; Γ ⊢ e0 : ~𝔹 /\
+    Σ; Γ ⊢ e1 : τ' /\
+    Σ; Γ ⊢ e2 : τ' /\
+    Σ; Γ ⊢ τ' :: *@O /\
+    Σ ⊢ τ ≡ τ'.
+Proof.
+  type_inv_solver.
+Qed.
+
+Lemma type_inv_proj Γ b e τ :
+  Σ; Γ ⊢ π@b e : τ ->
+  exists τ1 τ2,
+    Σ; Γ ⊢ e : τ1 * τ2 /\
+    Σ ⊢ τ ≡ ite b τ1 τ2.
+Proof.
+  type_inv_solver.
+Qed.
+
+Lemma type_inv_unfold Γ X e τ :
+  Σ; Γ ⊢ unfold<X> e : τ ->
+  exists τ',
+    Σ !! X = Some (DADT τ') /\
+    Σ; Γ ⊢ e : gvar X /\
+    Σ ⊢ τ ≡ τ'.
+Proof.
+  type_inv_solver.
+Qed.
+
+End inversion.
 
 Tactic Notation "apply_kind_inv" hyp(H) "by" tactic3(tac) :=
   lazymatch type of H with
@@ -210,229 +441,6 @@ Tactic Notation "apply_kind_inv" :=
 Tactic Notation "apply_kind_inv" "*" :=
   do_hyps (fun H => try dup_hyp H (fun H => apply_kind_inv H)).
 
-(** ** Type inversion *)
-Tactic Notation "type_inv_solver" "by" tactic3(tac) :=
-  match goal with
-  | |- _; _ ⊢ ?e : _ -> _ => remember e
-  end;
-  induction 1; subst; simp_hyps; simplify_eq;
-  tac.
-
-Tactic Notation "type_inv_solver" :=
-  type_inv_solver by (repeat esplit; eauto; equiv_naive_solver).
-
-Lemma type_inv_unit Σ Γ τ :
-  Σ; Γ ⊢ () : τ ->
-  Σ ⊢ τ ≡ 𝟙.
-Proof.
-  type_inv_solver.
-Qed.
-
-Lemma type_inv_lit Σ Γ b τ :
-  Σ; Γ ⊢ lit b : τ ->
-  Σ ⊢ τ ≡ 𝔹.
-Proof.
-  type_inv_solver.
-Qed.
-
-Lemma type_inv_abs Σ Γ e τ2 τ :
-  Σ; Γ ⊢ \:τ2 => e : τ ->
-  exists τ1 κ L,
-    Σ; Γ ⊢ τ2 :: κ /\
-    (forall x, x ∉ L -> Σ; (<[x:=τ2]> Γ) ⊢ e^x : τ1^x) /\
-    Σ ⊢ τ ≡ Π:τ2, τ1.
-Proof.
-  type_inv_solver.
-Qed.
-
-Lemma type_inv_gvar Σ Γ x τ :
-  Σ; Γ ⊢ gvar x : τ ->
-  exists τ' e,
-    Σ !! x = Some (DFun τ' e) /\
-    Σ ⊢ τ ≡ τ'.
-Proof.
-  type_inv_solver.
-Qed.
-
-Lemma type_inv_pair Σ Γ e1 e2 τ :
-  Σ; Γ ⊢ (e1, e2) : τ ->
-  exists τ1 τ2,
-    Σ; Γ ⊢ e1 : τ1 /\
-    Σ; Γ ⊢ e2 : τ2 /\
-    Σ ⊢ τ ≡ τ1 * τ2.
-Proof.
-  type_inv_solver.
-Qed.
-
-Lemma type_inv_inj Σ Γ b e τ' τ :
-  Σ; Γ ⊢ inj@b<τ'> e : τ ->
-  exists τ1 τ2 κ,
-    τ' = <{ τ1 + τ2 }> /\
-    Σ; Γ ⊢ τ1 + τ2 :: κ /\
-    Σ; Γ ⊢ e : ite b τ1 τ2 /\
-    Σ ⊢ τ ≡ τ1 + τ2.
-Proof.
-  type_inv_solver.
-Qed.
-
-Lemma type_inv_oinj Σ Γ b e τ' τ :
-  Σ; Γ ⊢ ~inj@b<τ'> e : τ ->
-  exists τ1 τ2,
-    τ' = <{ τ1 ~+ τ2 }> /\
-    Σ; Γ ⊢ τ1 ~+ τ2 :: *@O /\
-    Σ; Γ ⊢ e : ite b τ1 τ2 /\
-    Σ ⊢ τ ≡ τ1 ~+ τ2.
-Proof.
-  type_inv_solver.
-Qed.
-
-Lemma type_inv_fold Σ Γ X e τ :
-  Σ; Γ ⊢ fold<X> e : τ ->
-  exists τ',
-    Σ; Γ ⊢ e : τ' /\
-    Σ !! X = Some (DADT τ') /\
-    Σ ⊢ τ ≡ gvar X.
-Proof.
-  type_inv_solver.
-Qed.
-
-Lemma type_inv_boxedlit Σ Γ b τ :
-  Σ; Γ ⊢ [b] : τ ->
-  Σ ⊢ τ ≡ ~𝔹.
-Proof.
-  type_inv_solver.
-Qed.
-
-Lemma type_inv_boxedinj Σ Γ b v ω τ :
-  Σ; Γ ⊢ [inj@b<ω> v] : τ ->
-  exists ω1 ω2,
-    ω = <{ ω1 ~+ ω2 }> /\
-    ovalty <{ [inj@b<ω> v] }> ω /\
-    Σ ⊢ τ ≡ ω1 ~+ ω2.
-Proof.
-  type_inv_solver by hauto lq: on solve: equiv_naive_solver
-                           ctrs: ovalty inv: ovalty.
-Qed.
-
-Lemma type_inv_case Σ Γ e0 e1 e2 τ :
-  Σ; Γ ⊢ case e0 of e1 | e2 : τ ->
-  exists τ1 τ2 τ' κ L1 L2,
-    Σ; Γ ⊢ τ'^e0 :: κ /\
-    Σ; Γ ⊢ e0 : τ1 + τ2 /\
-    (forall x, x ∉ L1 -> Σ; (<[x:=τ1]> Γ) ⊢ e1^x : τ'^(inl<τ1 + τ2> x)) /\
-    (forall x, x ∉ L2 -> Σ; (<[x:=τ2]> Γ) ⊢ e2^x : τ'^(inr<τ1 + τ2> x)) /\
-    Σ ⊢ τ ≡ τ'^e0.
-Proof.
-  type_inv_solver.
-Qed.
-
-Lemma type_inv_ocase Σ Γ e0 e1 e2 τ :
-  Σ; Γ ⊢ ~case e0 of e1 | e2 : τ ->
-  exists τ1 τ2 τ' L1 L2,
-    Σ; Γ ⊢ τ' :: *@O /\
-    Σ; Γ ⊢ e0 : τ1 ~+ τ2 /\
-    (forall x, x ∉ L1 -> Σ; (<[x:=τ1]> Γ) ⊢ e1^x : τ') /\
-    (forall x, x ∉ L2 -> Σ; (<[x:=τ2]> Γ) ⊢ e2^x : τ') /\
-    Σ ⊢ τ ≡ τ'.
-Proof.
-  type_inv_solver.
-Qed.
-
-Lemma type_inv_case_ Σ Γ l e0 e1 e2 τ :
-  Σ; Γ ⊢ case{l} e0 of e1 | e2 : τ ->
-  exists τ1 τ2 τ' κ L1 L2,
-    Σ; Γ ⊢ τ' :: κ /\
-    Σ; Γ ⊢ e0 : τ1 +{l} τ2 /\
-    (forall x, x ∉ L1 -> exists τ', Σ; (<[x:=τ1]> Γ) ⊢ e1^x : τ') /\
-    (forall x, x ∉ L2 -> exists τ', Σ; (<[x:=τ2]> Γ) ⊢ e2^x : τ') /\
-    Σ ⊢ τ ≡ τ'.
-Proof.
-  type_inv_solver by (repeat (esplit; eauto); equiv_naive_solver).
-Qed.
-
-Lemma type_inv_prod Σ Γ τ1 τ2 τ :
-  Σ; Γ ⊢ τ1 * τ2 : τ -> False.
-Proof.
-  type_inv_solver.
-Qed.
-
-Lemma type_inv_sum Σ Γ l τ1 τ2 τ :
-  Σ; Γ ⊢ τ1 +{l} τ2 : τ -> False.
-Proof.
-  type_inv_solver.
-Qed.
-
-Lemma type_inv_app Σ Γ e1 e2 τ :
-  Σ; Γ ⊢ e1 e2 : τ ->
-  exists τ1 τ2,
-    Σ; Γ ⊢ e1 : Π:τ2, τ1 /\
-    Σ; Γ ⊢ e2 : τ2 /\
-    Σ ⊢ τ ≡ τ1^e2.
-Proof.
-  type_inv_solver.
-Qed.
-
-Lemma type_inv_let Σ Γ e1 e2 τ :
-  Σ; Γ ⊢ let e1 in e2 : τ ->
-  exists τ1 τ2 L,
-    Σ; Γ ⊢ e1 : τ1 /\
-    (forall x, x ∉ L -> Σ; (<[x:=τ1]> Γ) ⊢ e2^x : τ2^x) /\
-    Σ ⊢ τ ≡ τ2^e1.
-Proof.
-  type_inv_solver.
-Qed.
-
-Lemma type_inv_sec Σ Γ e τ :
-  Σ; Γ ⊢ s𝔹 e : τ ->
-  Σ; Γ ⊢ e : 𝔹 /\
-  Σ ⊢ τ ≡ ~𝔹.
-Proof.
-  type_inv_solver.
-Qed.
-
-Lemma type_inv_ite Σ Γ e0 e1 e2 τ :
-  Σ; Γ ⊢ if e0 then e1 else e2 : τ ->
-  exists τ' κ,
-    Σ; Γ ⊢ e0 : 𝔹 /\
-    Σ; Γ ⊢ e1 : τ'^(lit true) /\
-    Σ; Γ ⊢ e2 : τ'^(lit false) /\
-    Σ; Γ ⊢ τ'^e0 :: κ /\
-    Σ ⊢ τ ≡ τ'^e0.
-Proof.
-  type_inv_solver.
-Qed.
-
-Lemma type_inv_mux Σ Γ e0 e1 e2 τ :
-  Σ; Γ ⊢ ~if e0 then e1 else e2 : τ ->
-  exists τ',
-    Σ; Γ ⊢ e0 : ~𝔹 /\
-    Σ; Γ ⊢ e1 : τ' /\
-    Σ; Γ ⊢ e2 : τ' /\
-    Σ; Γ ⊢ τ' :: *@O /\
-    Σ ⊢ τ ≡ τ'.
-Proof.
-  type_inv_solver.
-Qed.
-
-Lemma type_inv_proj Σ Γ b e τ :
-  Σ; Γ ⊢ π@b e : τ ->
-  exists τ1 τ2,
-    Σ; Γ ⊢ e : τ1 * τ2 /\
-    Σ ⊢ τ ≡ ite b τ1 τ2.
-Proof.
-  type_inv_solver.
-Qed.
-
-Lemma type_inv_unfold Σ Γ X e τ :
-  Σ; Γ ⊢ unfold<X> e : τ ->
-  exists τ',
-    Σ !! X = Some (DADT τ') /\
-    Σ; Γ ⊢ e : gvar X /\
-    Σ ⊢ τ ≡ τ'.
-Proof.
-  type_inv_solver.
-Qed.
-
 Tactic Notation "apply_type_inv" hyp(H) "by" tactic3(tac) :=
   lazymatch type of H with
   | _; _ ⊢ () : _ => tac type_inv_unit
@@ -460,7 +468,10 @@ Tactic Notation "apply_type_inv" hyp(H) "by" tactic3(tac) :=
   end.
 
 Tactic Notation "apply_type_inv" hyp(H) :=
-  apply_type_inv H by (fun lem => apply lem in H; try simp_hyp H).
+  apply_type_inv H by (fun lem => apply lem in H; try simp_hyp H);
+  try lazymatch goal with
+      | |- gctx_wf _ => assumption
+      end.
 
 Tactic Notation "apply_type_inv" :=
   do_hyps (fun H => try apply_type_inv H).
